add some more rwlock transitions

concurrency/scache/FullMap.i.dfy
@@ -10,9 +10,28 @@ module FullMaps {
     imap k | true :: 0
   }
 
+  function unit_fn<A(!new)>(a: A) : FullMap<A, nat> {
+    imap k | true :: (if k == a then 1 else 0)
+  }
+
   function add_fns<A(!new)>(f: FullMap<A, nat>, g: FullMap<A, nat>) : FullMap<A, nat> {
     imap b | true :: f[b] + g[b]
   }
 
   function SumFilter<A(!new)>(fn: (A) -> bool, f: FullMap<A, nat>) : nat
+
+  lemma SumFilterSimp<A>()
+  ensures forall fn: (A) -> bool, f: FullMap<A, nat>, g: FullMap<A, nat>
+      {:trigger SumFilter(fn, add_fns(f, g)) } ::
+      SumFilter(fn, add_fns(f, g)) == SumFilter(fn, f) + SumFilter(fn, g)
+
+  ensures forall fn: (A) -> bool, x: A
+      {:trigger SumFilter(fn, unit_fn(x)) } ::
+      SumFilter(fn, unit_fn(x)) == (if fn(x) then 1 else 0)
+
+  ensures forall fn: (A) -> bool
+      {:trigger SumFilter(fn, zero_map()) } ::
+      SumFilter(fn, zero_map()) == 0
+  {
+  }
 }
